New representation using a universal type. Advantages: no longer need helpers, or different kinds of lookup and assign functions. Definitions become much simpler. Disadvantage so far: many theorems need to have a side condition (!v. (eject (inject v) = v)) for each type of v that enters the store.

hol/ptypesScript.sml
@@ -36,79 +36,50 @@ val _ = type_abbrev("Term", ``:(VarTerm + FunTerm)``);
 val _ = Hol_datatype `TempMultiequation = <| S : Term List ptr ; M : Term List ptr |>`;
 val _ = Hol_datatype `System = <| T : Multiequation List ptr ; U : Multiequation List ptr |>`;
 
-val _ = Hol_datatype `value
-= injectVariable of Variable
-| injectSetOfVariables of SetOfVariables
-| injectTerm of Term
-| injectTermAuxList of Term AuxList
-| injectTermList of Term List
-| injectMultiequation of Multiequation
-| injectMultiequationAuxList of Multiequation AuxList
-| injectMultiequationList of Multiequation List
-| injectTempMultiequation of TempMultiequation
-| injectTempMultiequationAuxList of TempMultiequation AuxList
-| injectTempMultiequationList of TempMultiequation List
-| injectSystem of System`;
-
-val ejectVariable_def = Define `ejectVariable (injectVariable a) = a`;
-val ejectSetOfVariables_def = Define `ejectSetOfVariables (injectSetOfVariables a) = a`;
-val ejectTerm_def = Define `ejectTerm (injectTerm a) = a`;
-val ejectTermAuxList_def = Define `ejectTermAuxList (injectTermAuxList a) = a`;
-val ejectTermList_def = Define `ejectTermList (injectTermList a) = a`;
-val ejectMultiequation_def = Define `ejectMultiequation (injectMultiequation a) = a`;
-val ejectMultiequationAuxList_def = Define `ejectMultiequationAuxList (injectMultiequationAuxList a) = a`;
-val ejectMultiequationList_def = Define `ejectMultiequationList (injectMultiequationList a) = a`;
-val ejectTempMultiequation_def = Define `ejectTempMultiequation (injectTempMultiequation a) = a`;
-val ejectTempMultiequationAuxList_def = Define `ejectTempMultiequationAuxList (injectTempMultiequationAuxList a) = a`;
-val ejectTempMultiequationList_def = Define `ejectTempMultiequationList (injectTempMultiequationList a) = a`;
-val ejectSystem_def = Define `ejectSystem (injectSystem a) = a`;
-val _ = export_rewrites [
-"ejectVariable_def",
-"ejectSetOfVariables_def",
-"ejectTerm_def",
-"ejectTermAuxList_def",
-"ejectTermList_def",
-"ejectMultiequation_def",
-"ejectMultiequationAuxList_def",
-"ejectMultiequationList_def",
-"ejectTempMultiequation_def",
-"ejectTempMultiequationAuxList_def",
-"ejectTempMultiequationList_def",
-"ejectSystem_def"];
+val _ = type_abbrev ("value",
+``:Variable
+ + SetOfVariables
+ + Term
+ + Term AuxList
+ + Term List
+ + Multiequation
+ + Multiequation AuxList
+ + Multiequation List
+ + TempMultiequation
+ + TempMultiequation AuxList
+ + TempMultiequation List
+ + System``);
 
 val _ = type_abbrev("store", ``:num |-> value``);
 
-val raw_lookup_def = Define` raw_lookup n = (λs:store. (FLOOKUP s n, s))`;
-val make_lookup_def = Define`
-  (make_lookup (eject:value -> 'a) (addr n : 'a ptr) = OPTIONT_BIND (raw_lookup n) (λv. OPTIONT_UNIT (eject v))) ∧
-  (make_lookup eject ptr = OPTIONT_FAIL)`;
-val _ = type_abbrev("lookup", ``:'a ptr -> store -> 'a option # store``);
+val embed_def = Define`
+  embed = @p. ∀x. (SND p) ((FST p) x : value) = x`
+val _ = overload_on ("inject", ``FST embed``);
+val _ = overload_on ("eject", ``SND embed``);
 
-val raw_assign_def = Define`raw_assign n v = (λs:store. ((), s |+ (n,v)))`;
-val make_assign_def = Define`
-  (make_assign (inject:'a -> value) (addr n : 'a ptr) v = do raw_assign n (inject v) ; return (addr n) od) ∧
-  (make_assign inject ptr v = return ptr)`;
-val _ = type_abbrev("assign", ``:'a ptr -> 'a -> store -> 'a ptr # store``);
+val embed_Term_thm = Q.store_thm(
+"embed_Term_thm",
+`eject (inject (v:Term)) = v`,
+srw_tac [][embed_def] >>
+SELECT_ELIM_TAC >> srw_tac [][] >>
+qexists_tac `(INR o INR o INL, OUTL o OUTR o OUTR)` >>
+srw_tac [][]);
 
-val _ = Hol_datatype `helpers = <| lookup : 'a lookup ; lookupList : 'a List lookup ; lookupAuxList : 'a AuxList lookup ;
-                                   assign : 'a assign ; assignList : 'a List assign ; assignAuxList : 'a AuxList assign |>`;
+val embed_Term_List_thm = Q.store_thm(
+"embed_Term_List_thm",
+`eject (inject (v:Term List)) = v`,
+srw_tac [][embed_def] >>
+SELECT_ELIM_TAC >> srw_tac [][] >>
+qexists_tac `(INR o INR o INR o INR o INL, OUTL o OUTR o OUTR o OUTR o OUTR)` >>
+srw_tac [][]);
 
-val valid_assign_lookup_def = Define`
-valid_assign_lookup assign lookup =
-  (∀a v s ptr' s'. (assign (pnil a) v s = (ptr', s')) ⇔ (ptr' = pnil a) ∧ (s' = s)) ∧
-  (∀ptr s vo s'. (lookup ptr s = (vo, s')) ⇒ (s' = s)) ∧
-  (∀ptr s. (lookup ptr s = (NONE, s)) ⇔ ((∃a. ptr = pnil a) ∨ (∃n. (ptr = addr n) ∧ n ∉ FDOM s))) ∧
-  (∀n v s ptr' s'. (assign (addr n) v s = (ptr', s')) ⇒
-                   (ptr' = addr n) ∧
-                   (s \\ n = s' \\ n) ∧
-                   (lookup (addr n) s' = (SOME v, s'))) ∧
-  (∀n s1 s2 v. (lookup (addr n) s1 = (SOME v, s1)) ∧ (FLOOKUP s1 n = FLOOKUP s2 n) ⇒ (lookup (addr n) s2 = (SOME v, s2)))`;
+val lookup_def = Define`
+  (lookup (addr n : 'a ptr) = OPTIONT_BIND (λs. (FLOOKUP s n, s)) (λv. OPTIONT_UNIT (eject:value->'a v))) ∧
+  (lookup pnil_ = OPTIONT_FAIL)`;
 
-val valid_helpers_def = Define`
-  valid_helpers h =
-  valid_assign_lookup h.assign h.lookup ∧
-  valid_assign_lookup h.assignAuxList h.lookupAuxList ∧
-  valid_assign_lookup h.assignList h.lookupList`;
+val assign_def = Define`
+  (assign (addr n : 'a ptr) v = (λs:store. ((), s |+ (n, inject:'a->value v)))) ∧
+  (assign pnil_ v = return ())`;
 
 val dispose_def = Define`
   (dispose (addr n) = (λs:store. ((), s \\ n))) ∧
@@ -117,63 +88,63 @@ val dispose_def = Define`
 val free_addr_def = Define`
   free_addr = λs:store. (addr (@n. n ∉ FDOM s), s)`;
 
-val new_def = Define`new assign v = do ptr <- free_addr ; assign ptr v od`;
+val new_def = Define`new v = do ptr <- free_addr ; assign ptr v ; return ptr od`;
 
 val CreateList_def = Define`
-  CreateList h =
-  do l <- new h.assignAuxList (AuxList (pnil ARB) (pnil ARB)) ;
-     s <- new h.assignList (List l l) ;
+  CreateList =
+  do l <- new (AuxList (pnil ARB) (pnil ARB)) ;
+     s <- new (List l l) ;
      return s
   od`;
 
 val HeadOfList_def = Define`
-  HeadOfList h (s:'a List ptr) =
-  do s' <- h.lookupList s ;
-     s'first' <- h.lookupAuxList s'.first ;
+  HeadOfList s =
+  do s' <- lookup s ;
+     s'first' <- lookup s'.first ;
      return s'first'.head
   od`;
 
 val EmptyList_def = Define`
-  EmptyList h (s : 'a List ptr) =
-  do s' <- h.lookupList s ;
+  EmptyList s =
+  do s' <- lookup s ;
      return (s'.first = s'.last)
   od`;
 
 val TailOfList_def = Define`
-  TailOfList h (s : 'a List ptr) =
-  do s' <- h.lookupList s ;
+  TailOfList s =
+  do s' <- lookup s ;
      l <- return s'.first ;
-     l' <- h.lookupAuxList l;
-     h.assignList s (List l'.tail s'.last) ;
+     l' <- lookup l;
+     assign s (List l'.tail s'.last) ;
      dispose l ;
      return s
   od`;
 
 val AddToEndOfList_def = Define`
-  AddToEndOfList h (t : 'a ptr) (s : 'a List ptr) =
-  do l <- new h.assignAuxList (AuxList (pnil ARB) (pnil ARB)) ;
-     s' <- h.lookupList s ;
-     h.assignAuxList s'.last (AuxList t l) ;
-     h.assignList s (List s'.first l) ;
+  AddToEndOfList t s =
+  do l <- new (AuxList (pnil ARB) (pnil ARB)) ;
+     s' <- lookup s ;
+     assign s'.last (AuxList t l) ;
+     assign s (List s'.first l) ;
      return s
   od`;
 
 val AddToFrontOfList_def = Define`
-  AddToFrontOfList h (t : 'a ptr) (s : 'a List ptr) =
-  do s' <- h.lookupList s ;
-     l <- new h.assignAuxList (AuxList t s'.first) ;
-     h.assignList s (List l s'.last) ;
+  AddToFrontOfList t s =
+  do s' <- lookup s ;
+     l <- new (AuxList t s'.first) ;
+     assign s (List l s'.last) ;
      return s
   od`;
 
 val AppendLists_def = Define`
-  AppendLists h (t1 : 'a List ptr) (t2 : 'a List ptr) =
-  do t2' <- h.lookupList t2 ;
+  AppendLists t1 t2 =
+  do t2' <- lookup t2 ;
      if t2'.first ≠ t2'.last then
-        do t1' <- h.lookupList t1 ;
-           t2'first' <- h.lookupAuxList t2'.first ;
-           h.assignAuxList t1'.last (AuxList t2'first'.head t2'first'.tail) ;
-           h.assignList t1 (List t1'.first t2'.last) ;
+        do t1' <- lookup t1 ;
+           t2'first' <- lookup t2'.first ;
+           assign t1'.last (AuxList t2'first'.head t2'first'.tail) ;
+           assign t1 (List t1'.first t2'.last) ;
            return ()
         od
      else return () ;
@@ -182,35 +153,15 @@ val AppendLists_def = Define`
      return t1
   od`;
 
-val OfTerms_def = Define`
-  OfTerms = <|
-  lookup := make_lookup ejectTerm ; lookupList := make_lookup ejectTermList ; lookupAuxList := make_lookup ejectTermAuxList ;
-  assign := make_assign injectTerm ; assignList := make_assign injectTermList ; assignAuxList := make_assign injectTermAuxList |>`;
-
-val valid_helpers_OfTerms = Q.store_thm(
-"valid_helpers_OfTerms",
-`valid_helpers OfTerms`,
-let
-val thms = [valid_helpers_def,valid_assign_lookup_def,OfTerms_def,make_assign_def,raw_assign_def,
-           make_lookup_def,IGNORE_BIND_DEF,BIND_DEF,UNIT_DEF,OPTIONT_BIND_def,raw_lookup_def,
-           FLOOKUP_UPDATE,OPTIONT_UNIT_def,OPTIONT_FAIL_def,FLOOKUP_DEF,EQ_IMP_THM]
-in
-srw_tac [] thms >>
-TRY (Cases_on `ptr`) >>
-fsrw_tac [] thms >>
-pop_assum mp_tac >> srw_tac [][] >>
-fsrw_tac [][]
-end);
-
 val (corresponding_list_rules, corresponding_list_ind, corresponding_list_cases) = Hol_reln`
-  (((EmptyList h ptr) s = (SOME T, s')) ⇒ corresponding_list h ptr s []) ∧
-  (((do hd <- HeadOfList h ptr ;
-        tl <- TailOfList h ptr ;
-        (hd':'a) <- h.lookup hd ;
+  (((EmptyList ptr) s = (SOME T, s')) ⇒ corresponding_list ptr s []) ∧
+  (((do hd <- HeadOfList ptr ;
+        tl <- TailOfList ptr ;
+        (hd':'a) <- lookup hd ;
         return (hd',tl)
      od) s = (SOME (hd',tl),s')) ∧
-   corresponding_list h tl s' tl' ⇒
-   corresponding_list h ptr s (hd'::tl'))`;
+   corresponding_list tl s' tl' ⇒
+   corresponding_list ptr s (hd'::tl'))`;
 
 val NOTIN_INFINITE_FDOM_exists = Q.store_thm(
 "NOTIN_INFINITE_FDOM_exists",
@@ -218,27 +169,26 @@ val NOTIN_INFINITE_FDOM_exists = Q.store_thm(
 PROVE_TAC [pred_setTheory.IN_INFINITE_NOT_FINITE,FDOM_FINITE]);
 val _ = export_rewrites["NOTIN_INFINITE_FDOM_exists"];
 
+val free_addr_elim_thm = Q.store_thm(
+"free_addr_elim_thm",
+`∀P s. (∀n. n ∉ FDOM s ⇒ P (addr n,s)) ⇒ P (free_addr s)`,
+srw_tac [][free_addr_def] >>
+SELECT_ELIM_TAC >>
+srw_tac [][]);
+
 val CreateList_creates_empty = Q.store_thm(
 "CreateList_creates_empty",
-`valid_helpers h ∧ (CreateList h s0 = (ptr, s)) ⇒ corresponding_list h ptr s []`,
-srw_tac [][CreateList_def,Once corresponding_list_cases,
-           BIND_DEF,UNIT_DEF] >>
-qexists_tac `s` >>
-qmatch_assum_abbrev_tac `UNCURRY f (new h.assignAuxList al s0) = (ptr,s)` >>
-Cases_on `new h.assignAuxList al s0` >>
-qmatch_assum_rename_tac `new h.assignAuxList al s0 = (ptr',s')` [] >>
-fsrw_tac [][pairTheory.UNCURRY,Abbr`f`] >>
-fsrw_tac [][new_def,BIND_DEF,UNIT_DEF,free_addr_def] >>
-`valid_assign_lookup h.assignAuxList h.lookupAuxList ∧
- valid_assign_lookup h.assignList h.lookupList` by PROVE_TAC [valid_helpers_def] >>
-qpat_assum `h.assignAuxList n al s0 = X` mp_tac >>
-SELECT_ELIM_TAC >> srw_tac [][] >>
-qmatch_assum_rename_tac `n ∉ FDOM s0` [] >>
-qpat_assum `h.assignList m l s' = X` mp_tac >>
-SELECT_ELIM_TAC >> srw_tac [][] >>
-qmatch_assum_rename_tac `m ∉ FDOM s'` [] >>
-`(ptr' = addr n) ∧ (h.lookupAuxList (addr n) s' = (SOME al, s'))` by metis_tac [valid_assign_lookup_def] >>
-`(ptr = addr m) ∧ (h.lookupList (addr m) s = (SOME (List ptr' ptr'), s))` by metis_tac [valid_assign_lookup_def] >>
-srw_tac [][EmptyList_def,BIND_DEF,UNIT_DEF,OPTIONT_BIND_def,OPTIONT_UNIT_def]);
+`(∀v. eject (inject (v:'a List)) = v) ⇒ (CreateList s0 = (ptr : 'a List ptr, s)) ⇒ corresponding_list ptr s []`,
+strip_tac >>
+simp_tac (srw_ss()) [CreateList_def,new_def,BIND_DEF] >>
+qho_match_abbrev_tac `(UNCURRY f (UNCURRY g (free_addr s0)) = (ptr,s)) ⇒ X` >>
+Q.ABBREV_TAC `P = (λx. (UNCURRY f (UNCURRY g x) = (ptr,s)) ⇒ X)` >>
+qsuff_tac `P (free_addr s0)` >- srw_tac [][Abbr`P`] >>
+ho_match_mp_tac free_addr_elim_thm >>
+srw_tac [][Abbr`P`,Abbr`g`,Abbr`f`,IGNORE_BIND_DEF,BIND_DEF,UNIT_DEF,assign_def,pairTheory.UNCURRY,Abbr`X`] >>
+Q.ABBREV_TAC `P = (λx. corresponding_list (FST x) (SND (assign (FST x) (List (addr n) (addr n)) (SND x))) [])`  >>
+qsuff_tac `P (free_addr (s0 |+ (n,inject (AuxList (pnil (ARB:'a)) (pnil ARB)))))` >- srw_tac [][Abbr`P`] >>
+ho_match_mp_tac free_addr_elim_thm >>
+srw_tac [][Abbr`P`,assign_def,Once corresponding_list_cases,EmptyList_def,OPTIONT_BIND_def,BIND_DEF,lookup_def,OPTIONT_UNIT_def,UNIT_DEF,FLOOKUP_UPDATE]);
 
 val _ = export_theory ()
